---
layout: post
title: 13-03 Dual norms
chapter: '13'
order: 4
owner: Wontak Ryu
categories:
- chapter13
lang: en
---
Let's examine an arbitrary **norm** $$\| x \|$$:

> $$l_p \text{ norm: } \lVert x \rVert_p = (\sum^n_{i=1} \rVert x_i \rVert_p)^{1/p}, \text{ for } p ≥ 1$$
>
> $$\text{Trace norm: } \lVert X \rVert_{tr} = \sum^r_{i=1} σ_i(X)$$


The **dual norm** of norm $$\lVert x \rVert$$ is denoted as $$\lVert x \rVert_{∗}$$ and is defined as follows:
 >$$\lVert x \rVert_{∗} = \max_{\lVert z \rVert ≤1} z^Tx$$


Suppose there exists some arbitrary $$y$$. Then when we let $$z = \frac{y}{\rVert y \rVert}$$, we have $$\rVert z \rVert = 1$$. Also, $$\rVert z^Tx \rVert \le \rVert x \rVert_{*}$$ holds,
therefore a form similar to the *Cauchy-Schwartz inequality* $$ \rVert y^Tx \rVert \le \rVert y \rVert \rVert x \rVert_{*} $$ is established.


Let's examine examples of dual norms under specific conditions:
> $$ l_p \text{ norm dual: } (\lVert x \rVert_p)_{*} = \lVert x \rVert_{q}, \text{ where } 1/p + 1/q = 1$$
>
> $$ \text{Trace norm dual: } (\lVert X \rVert_{tr})_{*} = \lVert X \rVert_{op}) = σ_1(X)$$

#### [Proof]
> Let's prove that the following holds for the $$ l_p$$ norm dual:
>
> $$(\lVert x \rVert_p)_{*} = \lVert x \rVert_{q}, \text{ where } 1/p + 1/q = 1 \qquad \text{(1)}$$
>
> *Proof*
>
> $$ (\lVert x \rVert_p)_{*} = \sup \{ z^Tx : x \in \mathbb{R}^n, \rVert x \rVert_q \le 1 \} \qquad  \text{(2)}$$
>
> Meanwhile, by Holder's inequality, the following holds:
>
> $$z^T x ≤ \rVert z^tx \rVert 1 ≤ \rVert z \rVert_p \rVert x \rVert_q (\text{ where }, 1/p + 1/q = 1)\qquad \text{(3)}$$
>
> From (1) above, the following relationship holds:
>
> $$(\rVert z \rVert_q)_∗ ≤ \rVert z \rVert_p\qquad \text{(4)}$$
>
> Therefore, if we find $$x$$ such that $$\rVert x \rVert_q ≤ 1$$ and $$z^Tx$$ satisfies $$\rVert z \rVert_p$$, we can see that $$(\rVert z \rVert_q)_∗ = \rVert z \rVert\rVert_p$$ holds.
>
> Meanwhile, if we set $$y := sign(z) \rVert z\rVert^{p−1} \left( y_i = sign(z_i)\rVert z_i\rVert^{p−1} \right)$$ and $$x = y$$, then $$\rVert y \rVert_q$$
> satisfies $$\rVert x \rVert_q =1$$, and we can confirm that $$z^Tx = \rVert z \rVert_p$$.
>
> Therefore, the following holds:
>
> $$( \rVert z \rVert_ q)_∗ = \rVert z \rVert_p, (1/p+1/q=1)\qquad \text{(5)}$$


The dual norm of a dual norm becomes the original norm again.
> $$\lVert x \rVert_{**} = \lVert x \rVert$$


Let's examine the following problem:
> $$ \min_y \lVert y \rVert \qquad \text{ subject to } y = x$$

When the optimal value is $$\rVert x \rVert$$, the Lagrangian is expressed as follows:

> $$L(y,u) = \rVert y \rVert+ u^T(x−y) = \rVert y \rVert − y^Tu + x^Tu$$

When expressed in terms of the dual norm $$(\lVert · \rVert_{∗})$$, it becomes:
> $$ \text{If } \rVert u \rVert_{∗} ≤ 1,\text{ then}  \qquad \min_y \{ \rVert y \rVert − y^Tu \} = 0 $$
>
> $$ \text{If } \rVert u \rVert_{∗} > 1, \text{ then}  \qquad \min_y \{ \rVert y \rVert − y^Tu \} = −∞ $$

### [Note]
> $$ \text{If } \rVert u \rVert_{∗} ≤ 1, \text{ then}  \qquad \min_y \{ \rVert y \rVert − y^Tu \} = 0 $$
>
> $$ \max_y (y^Tu - \rVert y \rVert ) = 0$$
>
> $$y^Tu \le \rVert y \rVert \rVert u \rVert_* \le \rVert y \rVert $$
>
> $$ \text{If } \rVert u \rVert_{∗} > 1, \text{ then}  \qquad \min_y \{ \rVert y \rVert − y^Tu \} = −∞ $$
>
> $$\text{Can always find} \qquad $$ $$z$$  with $$\rVert z \rVert = 1 \qquad \text{ subject to }\qquad z^Tu = \rVert u \rVert_{*} \qquad ( argmax_{\rVert z \rVert \le 1}  z^Tu )$$
>
> $$ \text{take} $$ $$y = t \cdot z, \qquad t > 0 $$
>
> $$ y^Tu = t \cdot \rVert u \rVert_{*} $$
>
> $$ \text{ for this } y, \qquad y^Tu - \rVert y \rVert = t \cdot \rVert u \rVert_{*} - t \rightarrow ∞ \text{ as } t \rightarrow ∞ $$
>
> $$ \text{ so therefore }  g(u) = \min_y L(y, u) = x^Tu - I(\rVert u \rVert_{*} \le 1)$$
>
> dual problem
>
> $$\max_u g(u) \iff \max_{\rVert u \rVert_{*} \le 1} x^Tu$$




Therefore, the Lagrange dual problem is as follows:

> $$ \max_u u^Tx \qquad \text{ subject to }\qquad \rVert u \rVert_{∗} ≤ 1$$

Since there are no inequality constraints, Slater's condition is satisfied, and according to strong duality, $$f^{\star} = g^{\star}$$.
That is, $$\rVert x \rVert = \rVert x \rVert_{∗∗}$$.
